Nemonuri/Executions/ExecutionFragment/Semantics/UniqueMem.lean
@@ -4,14 +4,14 @@ public import Nemonuri.Executions.ExecutionFragment.Semantics.Mem
 
 @[expose] public section
 
-namespace Nemonuri.TransitionSystem.ExecutionFragment.ExprRaw
+namespace Nemonuri.TransitionSystem.ExecutionFragment.SyntaxRaw
 
 variable {ts: TransitionSystem}
 
-def UniqueMem (coll elem: ts.FiniteExecutionFragmentRaw) : Prop := ExprRaw.Mem (.finite1 coll) (.finite elem)
+def UniqueMem (coll elem: ts.FiniteExecutionFragmentRaw) : Prop := Mem (.unique coll) (.finite elem)
 
 @[defeq]
-theorem uniqueMem_def {coll elem} : (@UniqueMem ts coll elem) = ExprRaw.Mem (.finite1 coll) (.finite elem) := rfl
+theorem uniqueMem_def {coll elem} : (@UniqueMem ts coll elem) = Mem (.unique coll) (.finite elem) := rfl
 
 
 namespace UniqueMem
@@ -20,7 +20,7 @@ variable {coll elem elem2: ts.FiniteExecutionFragmentRaw}
 
 --attribute [local simp low] uniqueMem_def
 
-theorem to_mem (h: UniqueMem coll elem) : ExprRaw.Mem (.finite1 coll) (.finite elem) := uniqueMem_def.mp h
+theorem to_mem (h: UniqueMem coll elem) : Mem (.unique coll) (.finite elem) := uniqueMem_def.mp h
 
 --theorem refl (fef: ts.FiniteExecutionFragmentRaw) (req: ts.IsFiniteExecutionFragment fef) : UniqueMem fef fef := Mem.finite1 (.mk fef req)
 
@@ -43,9 +43,17 @@ theorem trans (hl: UniqueMem coll elem) (hr: UniqueMem elem elem2) : UniqueMem c
 instance : IsTrans ts.FiniteExecutionFragmentRaw (@UniqueMem ts) := ⟨fun a b c => @UniqueMem.trans _ a b c⟩
 
 
-theorem to_refl (x: ts.FiniteExecutionFragmentRaw) (req: ts.IsFiniteExecutionFragment x) : UniqueMem x x := by
+theorem refl (x: ts.FiniteExecutionFragmentRaw) (req: ts.IsFiniteExecutionFragment x) : UniqueMem x x := by
   dsimp [uniqueMem_def]
-  exact Mem.finite1 (.mk x req)
+  exact Mem.unique (.mk x req)
+
+theorem refl_iff : UniqueMem elem elem ↔ ts.IsFiniteExecutionFragment elem := by
+  constructor
+  · intro lm1
+    dsimp [uniqueMem_def] at lm1
+    replace lm1 := lm1.is_executionFragment
+    cases lm1; assumption
+  · exact UniqueMem.refl _
 
 
 
@@ -66,6 +74,6 @@ theorem iff_eq (req: ts.IsFiniteExecutionFragment coll ∨ ts.IsFiniteExecutionF
 end UniqueMem
 
 
-end Nemonuri.TransitionSystem.ExecutionFragment.ExprRaw
+end Nemonuri.TransitionSystem.ExecutionFragment.SyntaxRaw
 
 end
