Nemonuri/Executions/ExecutionFragment/Syntax/Prefixes.lean
@@ -1,29 +1,29 @@
 module
 
-public import Nemonuri.Executions.ExecutionFragment.Expr.Raw
+public import Nemonuri.Executions.ExecutionFragment.Syntax.Raws
 
 @[expose] public section
 
-namespace Nemonuri.TransitionSystem.ExecutionFragment.ExprRaw
+namespace Nemonuri.TransitionSystem.ExecutionFragment.SyntaxRaw
 
 variable {ts: TransitionSystem}
 
 
-def pre : ExprRaw ts → ts.FiniteExecutionFragmentRaw
-  | .finite1 total => total
-  | .finite2 pre _ => pre
-  | .infinite1 pre => pre
+def pre : SyntaxRaw ts → ts.FiniteExecutionFragmentRaw
+  | .unique whole => whole
+  | .finites pre _ => pre
+  | .infinites pre => pre
 
 
 
 @[defeq, simp]
-theorem finite1_pre {x} : (@ExprRaw.finite1 ts x).pre = x := rfl
+theorem unique_pre {x} : (@SyntaxRaw.unique ts x).pre = x := rfl
 
 @[defeq, simp]
-theorem finite2_pre {x1 x2} : (@ExprRaw.finite2 ts x1 x2).pre = x1 := rfl
+theorem finites_pre {x1 x2} : (@SyntaxRaw.finites ts x1 x2).pre = x1 := rfl
 
 @[defeq, simp]
-theorem infinite1_pre {x} : (@ExprRaw.infinite1 ts x).pre = x := rfl
+theorem infinites_pre {x} : (@SyntaxRaw.infinites ts x).pre = x := rfl
 
 @[defeq, simp]
 theorem singleState_pre_states {s} : (@singleState ts s).pre.states = [s] := rfl
@@ -38,18 +38,18 @@ theorem ellipsis_pre_states : (@ellipsis ts).pre.states = [] := rfl
 theorem ellipsis_pre_actions : (@ellipsis ts).pre.actions = [] := rfl
 
 @[simp]
-theorem consEllipsis_pre_states {x} (req: x.toLabel = .finite1) : (@consEllipsis ts x).pre.states = [] := by
+theorem consEllipsis_pre_states {x} (req: x.toLabel = .unique) : (@consEllipsis ts x).pre.states = [] := by
   cases x <;> simp at req
   · rfl
 
 @[simp]
-theorem consEllipsis_pre_actions {x} (req: x.toLabel = .finite1) : (@consEllipsis ts x).pre.actions = [] := by
+theorem consEllipsis_pre_actions {x} (req: x.toLabel = .unique) : (@consEllipsis ts x).pre.actions = [] := by
   cases x <;> simp at req
   · rfl
 
 section StepL
 
-variable {tail: ExprRaw ts} {s: ts.S} {a: ts.Act}
+variable {tail: SyntaxRaw ts} {s: ts.S} {a: ts.Act}
 
 theorem stepL_pre_eq_pre_stepL : (stepL tail s a).pre = (tail.pre.stepL s a) := by
   cases tail <;> rfl
@@ -71,6 +71,6 @@ end StepL
 
 
 
-end Nemonuri.TransitionSystem.ExecutionFragment.ExprRaw
+end Nemonuri.TransitionSystem.ExecutionFragment.SyntaxRaw
 
 end
