Nemonuri/Executions/ExecutionFragment/Semantics/EvalToSet.lean
@@ -4,27 +4,28 @@ public import Nemonuri.Executions.ExecutionFragment.Semantics.Mem
 
 @[expose] public section
 
-namespace Nemonuri.TransitionSystem.ExecutionFragment.ExprRaw
+namespace Nemonuri.TransitionSystem.ExecutionFragment.SyntaxRaw
 
 variable {ts: TransitionSystem}
 
 
 
-def EvalToSet (coll: ExprRaw ts) : Set ts.ExecutionFragmentRaw := {elem | Mem coll elem}
+def EvalToSet (coll: SyntaxRaw ts) : Set ts.ExecutionFragmentRaw := {elem | Mem coll elem}
 
 namespace EvalToSet
 
-variable {coll: ExprRaw ts} {elem: ExecutionFragmentRaw ts}
+variable {coll: SyntaxRaw ts} {elem: ExecutionFragmentRaw ts}
 
 theorem mem_to_isExecutionFragment (h: elem ∈ coll.EvalToSet)
   : ts.IsExecutionFragment elem :=
-  ExprRaw.Mem.is_executionFragment h
+  SyntaxRaw.Mem.is_executionFragment h
 
 theorem mem_iff_mem : (elem ∈ coll.EvalToSet) ↔ Mem coll elem := by
   dsimp [EvalToSet]; rfl
 
+
 end EvalToSet
 
-end Nemonuri.TransitionSystem.ExecutionFragment.ExprRaw
+end Nemonuri.TransitionSystem.ExecutionFragment.SyntaxRaw
 
 end
